some more coq functional programming

coq_stuff/tutorial.v
@@ -1,6 +1,8 @@
 Set Implicit Arguments.
 Set Asymmetric Patterns.
 Require Import List.
+Require Import Bool.
+Require Import Arith_base.
 Open Scope list_scope.
 
 Inductive binop : Set :=
@@ -10,8 +12,8 @@ Inductive exp : Set :=
   | Const : nat -> exp
   | Binop : binop -> exp -> exp -> exp.
 (* take a binary operation and 2 expressions and return one expression *)
-Fixpoint frs (e1 : nat) (e2 : nat) : nat := e1.
-Fixpoint snd (e1 : nat) (e2 : nat) : nat := e2.
+Definition frs (e1 : nat) (e2 : nat) : nat := e1.
+Definition snd (e1 : nat) (e2 : nat) : nat := e2.
 
 Definition binopDenote := fun b =>
   match b with
@@ -57,7 +59,7 @@ Fixpoint progDenote (p : prog) (s : stack) : option stack :=
       | Some s' => progDenote p' s'
       end
   end.
-(* kinda cool how all binary instructions just generalize in the stack machine [they did not but now they do!] *)
+
 
 Fixpoint compile (e : exp) : prog :=
   match e with
@@ -67,17 +69,114 @@ Fixpoint compile (e : exp) : prog :=
 
 Eval simpl in compile (Const 42).
 Eval simpl in progDenote (compile (Binop Times (Binop Second(Const 2) (Const 3)) (Const 7))).
-(* yay! *)
 
-Lemma compile_correct' : forall e p s, progDenote (compile e ++ p) s = progDenote p (expDenote e :: s).
-induction e. intros. unfold compile. unfold expDenote. unfold progDenote at 1. simpl. fold progDenote. reflexivity.
-intros. unfold compile. fold compile. unfold expDenote. fold expDenote. rewrite app_assoc_reverse. rewrite IHe2.
-rewrite app_assoc_reverse. rewrite IHe1. unfold progDenote at 1. simpl. fold progDenote. reflexivity.
-Qed.
+
+Lemma compile_correct' : forall e p s, progDenote (compile e ++ p) s =
+  progDenote p (expDenote e :: s). induction e. intros. unfold compile. unfold
+  expDenote. unfold progDenote at 1. simpl. fold progDenote. reflexivity.
+  intros. unfold compile. fold compile. unfold expDenote. fold expDenote. rewrite
+  app_assoc_reverse. rewrite IHe2. rewrite app_assoc_reverse. rewrite IHe1.
+  unfold progDenote at 1. simpl. fold progDenote. reflexivity. Qed.
 Lemma nr : forall e, compile e = compile e ++ nil.
 intros. rewrite app_nil_r. reflexivity.
 Qed.
 Theorem compile_correct : forall e, progDenote (compile e) nil = Some (expDenote e :: nil).
 intros. rewrite nr. rewrite compile_correct'. reflexivity.
 Qed.
+
+
+
+Inductive arith : Set :=
+  | Nt : nat -> arith
+  | Ad : arith -> arith -> arith
+.
+Fixpoint evaluate (a : arith) : option arith :=
+  match a with
+  | Nt n => Some (Nt n)
+  | Ad n1 n2 =>
+      let s1 := evaluate n1 in
+      let s2 := evaluate n2 in
+      match s1 with
+      | Some (Nt new1) => match s2 with
+                    | Some (Nt new2) => Some (Nt (plus new1 new2))
+                    | _ => None
+                           end
+      | _ => None
+      end
+  end.
+  (* let a be Nat n for case 1
+     for case 2, open the definition and induct on (n1, n2). Base case is that they are both
+     natural numbers then it is simple that we get a natural number. If they are both not natural numbers,
+     then by the inductive hypothesis their evaluation is a natural number, so actually we are done.
+   *)
+
+Theorem reduces : forall e, exists n, evaluate e = Some (Nt n).
+Proof.
+  intros. unfold evaluate. case e. Abort.
+
+Inductive term : Set :=
+  | Nat : nat -> term
+  | True : term
+  | False : term
+  | Add : term -> term -> term
+  | And : term -> term -> term.
+
+Definition my_and (t1 : term) (t2 : term) : option term :=
+  match t1 with
+  | True => match t2 with
+              | True => Some True
+              | False => Some False
+              | _ => None  end
+  | False => Some False
+  | _ => None 
+  end.
+Fixpoint eval (t : term) : option term :=
+  match t with
+  | Nat n => Some (Nat n)
+  | True => Some True
+  | False => Some False
+  | Add n1 n2 => let s1 := eval n1 in
+      let s2 := eval n2 in
+      match s1 with
+      | Some (Nat new1) => match s2 with
+                          |  Some (Nat new2) => Some (Nat (plus new1 new2))
+                          | _ => None
+                           end
+      | _ => None
+      end
+  | And n1 n2 => let s1 := eval n1 in
+      let s2 := eval n2 in
+      my_and n1 n2
+  end.
+
+Inductive type_term : Set :=
+  | Bool
+  | Natural.
+Fixpoint typecheck (t: term) : option type_term :=
+  match t with
+  | Nat n => Some Natural
+  | True => Some Bool
+  | False => Some Bool
+  | Add n1 n2 => 
+      let s1 := typecheck n1 in
+      let s2 := typecheck n2 in
+      match (s1, s2) with
+      | (Some Natural, Some Natural) => Some Natural
+      | _ => None
+      end
+  | And n1 n2 =>
+      let s1 := typecheck n1 in
+      let s2 := typecheck n2 in
+      match (s1, s2) with
+      | (Some Bool, Some Bool) => Some Bool
+      | _ => None
+      end
+  end.
+
+Eval simpl in typecheck (Add (Add (Nat 5) (Nat 7)) (True)).
+
+Theorem type_sound : forall e, (exists a, typecheck e = Some a) -> 
+  (exists b, eval e = Some b).
+Proof.
+  intros. Abort.
 
